WIP

src/TU_to_Core.v
@@ -4,28 +4,50 @@ Require Import PArith.
 Module S := TaggedUnions.  
 Module T := Core. 
 
-Class Eqb (X : Type) := {eqb : X -> X -> bool; 
-                         eqb_correct: forall x y, Bool.reflect (x = y) (eqb x y) }. 
+
+Definition fin_of_var {T} l (t : T) : var l t -> Finite.T (List.length l).
+induction 1.
+refine  (Finite.Build_T _ 0 _). simpl. admit.
+refine  (Finite.Build_T _ (S (Finite.val IHX)) _). simpl. admit.
+Defined.
+
+Class Ordered  (X : Type) := {compare : X -> X -> comparison}.  
+
+Local Notation lex e f := (match e with Eq => f | _ => e end).
+
 
 Module M. 
-  Section t. 
-    Context (X : Type) {E : Eqb X}. 
-    Definition T := list (positive * X). 
   
-    Definition singleton x : T := ([(1%positive,x)])%list. 
+  Section t. 
+    Variable X : Type. 
+    Context {O : Ordered X}. 
+    
+    
 
+    Definition T := list (positive * X). 
+    
+    Definition singleton x : T := ([(1%positive,x)])%list. 
+    
     Fixpoint add n x (l : T) : T :=
       match l with 
         | nil => [(n,x)]
         | (m,y)::q => 
-            if eqb x y then ((n + m)%positive, x) :: q  else (m,y) :: add n x q
+            match compare x y with 
+              | Lt => (n, x) :: l
+              | Eq => (n+m,x)%positive :: q 
+              | Gt => (m,y):: add n x q
+            end
       end%list. 
 
     Fixpoint max n x (l : T) : T :=
       match l with 
         | nil => [(n,x)]
         | (m,y)::q => 
-            if eqb x y then (Pos.max n m, x) :: q  else (m,y) :: add n x q
+            match compare x y with 
+              | Lt => (n, x) :: l
+              | Eq => (Pos.max n m,x)%positive :: q 
+              | Gt => (m,y):: max n x q
+            end
       end%list. 
     
     Fixpoint union (a b : T) : T :=
@@ -37,7 +59,7 @@ Module M.
     Fixpoint join (a b : T) : T :=
       match a with 
         |nil => b 
-        | (n,x) :: q => max n x (union q b)
+        | (n,x) :: q => max n x (join q b)
       end%list. 
     
     Fixpoint copy n (x : X)  :=
@@ -69,36 +91,78 @@ Module M.
 
 End M. 
 
+Definition type0_cmp t t' := 
+  match t , t' with 
+    | Tunit, Tunit => Eq
+    | Tbool, Tbool => Eq
+    | Tint n , Tint m => NPeano.Nat.compare n m 
+    | Tfin n , Tfin m => NPeano.Nat.compare n m 
+
+    | Tunit, _ => Lt
+    | _, Tunit => Gt
+
+    | Tbool, _ => Lt
+    | _, Tbool => Gt
+
+    | Tint _, _ => Lt
+    | _, Tint _ => Gt
+
+    | Tfin _, _ => Lt
+    | _, Tfin _ => Gt       
+
+    | Tabstract _ _, _ => Lt
+  end. 
+
+Fixpoint type_cmp  t t' {struct t} :=
+  match t, t' with 
+      | T.Tlift t, T.Tlift t' => type0_cmp t t'
+      | T.Ttuple l, T.Ttuple l' => 
+          let list_compare := fix list_compare h k :=
+              match h,k with 
+                | nil, nil => Eq
+                | nil, _ => Lt
+                | _, nil => Gt
+                | cons t q, cons t' q' => lex (type_cmp t t') (list_compare q q')
+              end in 
+
+          list_compare l l' 
+      | T.Tlift _, _ => Lt
+      | _,  T.Tlift _ => Gt
+  end. 
+
 Section compile. 
   Variable Phi : S.state. 
+  
 
-  Instance Ttype_Eqb : Eqb T.type. 
-  Admitted. 
+  Instance Ord : Ordered T.type. 
+  refine  (Build_Ordered _ type_cmp). 
+  Defined. 
+
+  Definition open (x :  T.type) : M.T T.type :=
+    match x with 
+      | T.Tlift t0 => M.singleton (T.Tlift t0)
+      | T.Ttuple l => M.of_list l
+    end. 
+
   
   Definition flat : S.type -> T.type .
   intros x. 
-  Definition open : T.type -> M.T T.type. 
-  intros x. 
-  refine (
-      match x with 
-        | T.Tlift t0 => M.singleton (T.Tlift t0)
-        | T.Ttuple l => M.of_list l
-      end). 
-  Defined. 
   refine (
       let f := fix convert (x : S.type) : T.type :=
           match x with 
                   | S.Tlift t0 => T.Tlift t0
                   | S.Ttuple l => T.Ttuple (List.map convert l)
                   | S.Tunion C =>  
-                      let l := List.map convert C in 
-                      let l := List.map open l in 
-                      let m := List.fold_right M.join nil l in 
-                      let c := T.Tlift (Tfin (List.length C )) in 
-                        T.Ttuple (c:: M.contents _ m)
+                            let l := List.map convert C in 
+                            let l := List.map open l in 
+                            let m := List.fold_right M.join nil l in 
+                            let c := T.Tlift (Tfin (List.length C )) in 
+                              T.Ttuple (c:: M.contents _ m)
+
           end in _). 
   apply (f x). 
   Defined. 
+
   Definition compile_sync : S.sync -> T.sync. 
   Proof. 
     refine (fun X => match X with
@@ -106,17 +170,119 @@ Section compile.
                       |S.Tregfile n t => T.Tregfile n (flat t)
             end). 
   Defined. 
+
   Definition var_map { A B } (f : A -> B) l (t : A) : var l t -> var (List.map f l) (f t). 
   Admitted. 
+
   Definition compile_state : S.state -> T.state := List.map compile_sync. 
 
 
   Variable (R : T.type -> Type). 
+  Definition A := S.Tlift Tbool. 
+
+  Eval compute in flat (S.Tunion [ S.Tunion [A;A]; A]). 
+  Eval compute in flat (S.Tunion [ S.Tunion [A;A]; S.Tunion [S.Ttuple [A ; A] ; A; A]]). 
+  Eval compute in flat (S.Tunion [ S.Tunion [A;A]; S.Tunion [A;A]; S.Tunion [S.Ttuple [A ; A] ; A; A]]). 
+
+  (** Allocate takes the constructor [c] applied to [x], and return
+  the corresponding tuple. 
+
+  - The first element of the tuple correspond to the number of the
+    constructor.
+
+  - If t is a base type, then t must appear in |l| since we have [var
+    t l].
+
+  - If t is a tagged union, then it is being torn appart recursively,
+  and generates a tuple. It suffices to map this tuple to the bigger
+  tuple generated by [l]
+
+  - If it is a tuple, it suffices to map this tuple to the bigger
+    tuple generated by [l]
+
+ *)
+
+    
+    Definition Eapp l1 l2 : 
+      T.expr R (T.Ttuple l1) -> T.expr R (T.Ttuple l2) -> 
+      T.expr R (T.Ttuple (l1 ++ l2)).  
+    Admitted. 
+    Definition Eskip l1 l2 : 
+      T.expr R (T.Ttuple (l1 ++ l2)) -> T.expr R (T.Ttuple (l2)).  
+    Admitted. 
+    Definition Efirst l1 l2 : 
+      T.expr R (T.Ttuple (l1 ++ l2)) -> T.expr R (T.Ttuple (l1)).     
+    Admitted. 
+    
+    Definition Enull  t : T.expr R t. Admitted.  
+    
+    Definition Econs t l : 
+      T.expr R t -> T.expr R (T.Ttuple l) -> 
+      T.expr R (T.Ttuple (t::l)).  
+    Admitted. 
+
+  Section t. 
+    Notation MS := (M.T T.type). 
+    Inductive layout : MS -> MS -> Type :=
+    | layout_nil : forall l, layout nil l
+    | layout_cons : forall n m x q q', layout q q' -> 
+                                   (n <= m)%positive ->  
+                                  layout ((n,x) :: q)%list ((m, x):: q')%list
+    | layout_drop : forall n x q q', layout q q' -> 
+                                layout q ((n,x) :: q')%list. 
+
+    Definition apply_layout m1 m2 (H : layout m1 m2) (x : T.expr R (T.Ttuple (M.contents _ m1))) : T.expr R (T.Ttuple (M.contents _ m2)). 
+    induction H. 
+    + apply Enull. 
+    +  simpl. 
+    apply Eapp.  2: apply IHlayout. simpl in x. 
+    apply Efirst in x. clear - x l.  admit.  
+    simpl in x. apply Eskip in x. apply x.
+    + simpl. apply Eapp. 
+   
+    apply Enull. 
+    auto.
+    Defined. 
 
   Definition allocate t l (c : var l t) (x : T.expr R (flat t)) : T.expr R (flat (S.Tunion l)). 
   Proof. 
-  Admitted. 
+    simpl flat. 
+    apply Econs. 
+    apply T.Econstant. apply (fin_of_var _ _  c).
 
+    eapply (apply_layout ((M.singleton (flat t)))). 
+    Focus 2. simpl. apply T.Etuple. constructor. apply x. constructor. 
+    clear x.
+    Program Fixpoint try_layout m1 m2 : option (layout m1 m2) :=
+      match m1 with 
+        | nil => Some (layout_nil m2)
+        | (n,x)::q => match m2 with 
+                       | nil => None
+                       | (m,y) :: q' => match type_cmp x y with 
+                                        | Lt => None
+                                        | Eq => if Pos.ltb n m then 
+                                                 do l <- try_layout q q';
+                                                 _
+                                               else 
+                                                 None
+                                        | Gt => 
+                                            do l <- try_layout ((n,x)::q) q';
+                                            Some (layout_drop m y ((n,x)::q) q' l) : 
+                                            option (layout ((n,x)::q) ((m,y)::q'))
+                                       end
+                     end
+
+      end%list. 
+    Next Obligation. 
+      apply Some. 
+      apply layout_cons. 
+      refine Some (layout_cons n m x q q' l admit ):
+      option (layout (n,) m2)
+ 
+    induction l. simpl. inversion c.
+    simpl. 
+    simpl. 
+    apply T.Etuple. constructor. 
   Definition deallocate t l tr (c : var l t) (e : T.expr R (flat (S.Tunion l))) 
                         (cont : R (flat t) -> T.action (compile_state Phi) R (flat tr)): 
     T.action (compile_state Phi) R (flat tr). 
@@ -153,11 +319,6 @@ Section compile.
   apply (allocate _ _ c (compile _ x)). 
   Defined. 
 
-  Definition fin_of_var {T} l (t : T) : var l t -> Finite.T (List.length l).
-  induction 1.
-  refine  (Finite.Build_T _ 0 _). simpl. admit.
-  refine  (Finite.Build_T _ (S (Finite.val IHX)) _). simpl. admit.
-  Defined.
 
   Definition compile   t : S.action Phi (fun x => R (flat x )) t -> T.action (compile_state Phi ) R (flat t). 
   refine (let compile := fix compile t (a : S.action Phi (fun x => R (flat x)) t) : 
